theories/StretchPRG.v
@@ -55,114 +55,109 @@ Definition mkpair {Lt Lf E}
   (t: package Lt [interface] E) (f: package Lf [interface] E):
   loc_GamePair E := fun b => if b then {locpackage t} else {locpackage f}.
 
-Definition PRG1_pkg_tt:
-  package fset0
-    [interface]
+Definition GEN_pkg_tt:
+  package fset0 [interface]
     [interface #val #[query]: 'unit → 'word × 'word ] :=
   [package
-      #def #[query] (_: 'unit): 'word × 'word {
-        s <$ uniform Word_N ;;
-        ret (PRG s)
-      }
+    #def #[query] (_: 'unit): 'word × 'word {
+      s <$ uniform Word_N ;;
+      ret (PRG s)
+    }
   ].
 
-Definition PRG1_pkg_ff:
-  package fset0
-    [interface]
+Definition GEN_pkg_ff:
+  package fset0 [interface]
     [interface #val #[query]: 'unit → 'word × 'word ] :=
   [package
-      #def #[query] (_: 'unit): 'word × 'word {
-        r1 <$ uniform Word_N ;;
-        r2 <$ uniform Word_N ;;
-        ret (r1, r2)
-      }
+    #def #[query] (_: 'unit): 'word × 'word {
+      r1 <$ uniform Word_N ;;
+      r2 <$ uniform Word_N ;;
+      ret (r1, r2)
+    }
   ].
 
-Definition PRG1 := mkpair PRG1_pkg_tt PRG1_pkg_ff.
+Definition GEN := mkpair GEN_pkg_tt GEN_pkg_ff.
 
-Definition PRG2_pkg_tt:
-  package fset0
-    [interface]
+Definition GEN_STRETCH_pkg_tt:
+  package fset0 [interface]
     [interface #val #[query]: 'unit → 'word × 'word × 'word ] :=
   [package
-      #def #[query] (_: 'unit): 'word × 'word × 'word {
-        s <$ uniform Word_N ;;
-        let '(x, y) := PRG s in
-        ret (x, PRG y)
-      }
+    #def #[query] (_: 'unit): 'word × 'word × 'word {
+      s <$ uniform Word_N ;;
+      let '(x, y) := PRG s in
+      ret (x, PRG y)
+    }
   ].
 
-Definition PRG2_pkg_ff:
-  package fset0
-    [interface]
+Definition GEN_STRETCH_pkg_ff:
+  package fset0 [interface]
     [interface #val #[query]: 'unit → 'word × 'word × 'word ] :=
   [package
-      #def #[query] (_: 'unit): 'word × 'word × 'word {
-        x <$ uniform Word_N ;;
-        u <$ uniform Word_N ;;
-        v <$ uniform Word_N ;;
-        ret (x, (u, v))
-      }
+    #def #[query] (_: 'unit): 'word × 'word × 'word {
+      x <$ uniform Word_N ;;
+      u <$ uniform Word_N ;;
+      v <$ uniform Word_N ;;
+      ret (x, (u, v))
+    }
   ].
 
-Definition PRG2 := mkpair PRG2_pkg_tt PRG2_pkg_ff.
+Definition GEN_STRETCH := mkpair GEN_STRETCH_pkg_tt GEN_STRETCH_pkg_ff.
 
-Definition PRG2_HYB_pkg_1:
+Definition GEN_STRETCH_HYB_pkg_1:
   package fset0
     [interface #val #[query]: 'unit → 'word × 'word ]
     [interface #val #[query]: 'unit → 'word × 'word × 'word ] :=
   [package
-      #def #[query] (_: 'unit): 'word × 'word × 'word {
-        #import {sig #[query]: 'unit → 'word × 'word } as query ;;
-        xy ← query tt ;;
-        let '(x, y) := xy in
-        ret (x, PRG y)
-      }
+    #def #[query] (_: 'unit): 'word × 'word × 'word {
+      #import {sig #[query]: 'unit → 'word × 'word } as query ;;
+      '(x, y) ← query tt ;;
+      ret (x, PRG y)
+    }
   ].
 
-Definition PRG2_HYB_pkg_2:
+Definition GEN_STRETCH_HYB_pkg_2:
   package fset0
     [interface #val #[query]: 'unit → 'word × 'word ]
     [interface #val #[query]: 'unit → 'word × 'word × 'word ] :=
   [package
-      #def #[query] (_: 'unit): 'word × 'word × 'word {
-        #import {sig #[query]: 'unit → 'word × 'word } as query ;;
-        x <$ uniform Word_N ;;
-        uv ← query tt ;;
-        ret (x, uv)
-      }
+    #def #[query] (_: 'unit): 'word × 'word × 'word {
+      #import {sig #[query]: 'unit → 'word × 'word } as query ;;
+      x <$ uniform Word_N ;;
+      uv ← query tt ;;
+      ret (x, uv)
+    }
   ].
 
-Lemma PRG_equiv_true:
-  PRG2 true ≈₀ PRG2_HYB_pkg_1 ∘ PRG1 true.
+Lemma GEN_equiv_true:
+  GEN_STRETCH true ≈₀ GEN_STRETCH_HYB_pkg_1 ∘ GEN true.
 Proof.
   apply: eq_rel_perf_ind_eq.
   simplify_eq_rel m.
-  all: apply rpost_weaken_rule with eq.
-  2: by move=> [? ?] [? ?] [].
+  apply rpost_weaken_rule with eq;
+    last by move=> [? ?] [? ?] [].
   simplify_linking.
   ssprove_code_simpl.
   by apply: rreflexivity_rule.
 Qed.
 
-Lemma PRG_HYB_equiv:
-  PRG2_HYB_pkg_1 ∘ PRG1 false ≈₀ PRG2_HYB_pkg_2 ∘ PRG1 true.
+Lemma GEN_HYB_equiv:
+  GEN_STRETCH_HYB_pkg_1 ∘ GEN false ≈₀ GEN_STRETCH_HYB_pkg_2 ∘ GEN true.
 Proof.
   apply: eq_rel_perf_ind_eq.
   simplify_eq_rel m.
-  all: apply rpost_weaken_rule with eq.
-  2: by move=> [? ?] [? ?] [].
+  apply rpost_weaken_rule with eq;
+    last by move=> [? ?] [? ?] [].
   simplify_linking.
   by apply: rreflexivity_rule.
 Qed.
 
-Lemma PRG_equiv_false:
-  PRG2_HYB_pkg_2 ∘ PRG1 false ≈₀ PRG2 false.
+Lemma GEN_equiv_false:
+  GEN_STRETCH_HYB_pkg_2 ∘ GEN false ≈₀ GEN_STRETCH false.
 Proof.
   apply: eq_rel_perf_ind_eq.
   simplify_eq_rel m.
-  all: apply rpost_weaken_rule with eq.
-  2: by move=> [? ?] [? ?] [].
+  apply rpost_weaken_rule with eq;
+    last by move=> [? ?] [? ?] [].
   simplify_linking.
   by apply: rreflexivity_rule.
 Qed.
@@ -174,31 +169,31 @@ Local Open Scope ring_scope.
   which an adversary can distinguish the PRG from truly random numbers.
   Negligible by assumption.
 *)
-Definition prg_epsilon := Advantage PRG1.
+Definition prg_epsilon := Advantage GEN.
 
 Theorem security_based_on_prf LA A:
   ValidPackage LA
     [interface #val #[query]: 'unit → 'word × 'word × 'word ]
     A_export A ->
-  Advantage PRG2 A <=
-  prg_epsilon (A ∘ PRG2_HYB_pkg_1) +
-  prg_epsilon (A ∘ PRG2_HYB_pkg_2).
+  Advantage GEN_STRETCH A <=
+  prg_epsilon (A ∘ GEN_STRETCH_HYB_pkg_1) +
+  prg_epsilon (A ∘ GEN_STRETCH_HYB_pkg_2).
 Proof.
   move=> vA.
   rewrite Advantage_E Advantage_sym.
-  ssprove triangle (PRG2 true) [::
-    PRG2_HYB_pkg_1 ∘ PRG1 true ;
-    PRG2_HYB_pkg_1 ∘ PRG1 false ;
-    PRG2_HYB_pkg_2 ∘ PRG1 true ;
-    PRG2_HYB_pkg_2 ∘ PRG1 false
-  ] (PRG2 false) A
+  ssprove triangle (GEN_STRETCH true) [::
+    GEN_STRETCH_HYB_pkg_1 ∘ GEN true ;
+    GEN_STRETCH_HYB_pkg_1 ∘ GEN false ;
+    GEN_STRETCH_HYB_pkg_2 ∘ GEN true ;
+    GEN_STRETCH_HYB_pkg_2 ∘ GEN false
+  ] (GEN_STRETCH false) A
   as ineq.
   apply: le_trans.
   1: by apply: ineq.
-  rewrite PRG_equiv_true ?fdisjointUr ?fdisjoints0 // GRing.add0r.
-  rewrite PRG_HYB_equiv ?fdisjointUr ?fdisjoints0 // GRing.addr0.
-  rewrite PRG_equiv_false ?fdisjointUr ?fdisjoints0 // GRing.addr0.
-  by rewrite /prg_epsilon !Advantage_E -!Advantage_link !(Advantage_sym (PRG1 true)).
+  rewrite GEN_equiv_true ?fdisjointUr ?fdisjoints0 // GRing.add0r.
+  rewrite GEN_HYB_equiv ?fdisjointUr ?fdisjoints0 // GRing.addr0.
+  rewrite GEN_equiv_false ?fdisjointUr ?fdisjoints0 // GRing.addr0.
+  by rewrite /prg_epsilon !Advantage_E -!Advantage_link !(Advantage_sym (GEN true)).
 Qed.
 
 End StretchPRG_example.
